FoldTest.v
@@ -1,0 +1,28 @@
+Require Import List.
+Import ListNotations.
+
+Check fold_left.
+
+Definition f : list nat -> nat -> list nat :=
+  fun l (n:nat) => (l ++ [n]).
+
+Lemma fold_monotonic : forall prefix ns tr,
+  fold_left f ns [] = tr ->
+  fold_left f ns prefix = (prefix ++ tr).
+Proof.
+
+  (*
+  intros.
+  generalize dependent tr.
+  generalize dependent prefix.
+  induction ns; intros; simpl in *.
+  - inversion H; subst. rewrite app_nil_r. trivial.
+  - 
+    rewrite <- IHns.
+    unfold f. simpl. fold f.*)
+Abort.
+
+    
+    
+  
+  
