foo.v
@@ -1,0 +1,71 @@
+Require Import List.
+Import ListNotations.
+
+Definition snoc : list nat -> nat -> list nat :=
+  fun l n => l ++ [n].
+
+Theorem foo : forall l m,
+  fold_left snoc l m = m ++ l.
+Proof.
+  induction l as [|h t IH]; simpl; intro m.
+  - rewrite app_nil_r. reflexivity.
+  - unfold snoc; fold snoc.
+    assert (m ++ h :: t = (m ++ [h]) ++ t).
+    { rewrite <- app_assoc. reflexivity. }
+    rewrite H.
+    apply IH.
+Qed.
+
+Lemma fold_monotonic_gen : forall prefix ns tr l,
+    fold_left snoc ns l = tr ->
+    fold_left snoc ns prefix = prefix ++ (skipn (length l) tr).
+Proof.
+  intros prefix ns tr l H.
+  rewrite foo in H. subst.
+  assert (skipn (length l) (l ++ ns) = ns).
+  Search skipn.
+  admit.
+  rewrite H.
+  rewrite foo. reflexivity.
+Admitted.
+
+  
+ 
+Lemma fold_monotonic' : forall prefix ns tr,
+  fold_left snoc ns [] = tr ->
+  fold_left snoc ns prefix = prefix ++ tr.
+Proof.
+  intros.
+  assert (tr = (skipn (length ([]:list nat)) tr)).
+  auto.
+  rewrite H0.
+  apply fold_monotonic_gen. assumption.
+Defined.
+
+Lemma fold_monotonic : forall prefix ns tr,
+  fold_left snoc ns [] = tr ->
+  fold_left snoc ns prefix = prefix ++ tr.
+Proof.
+  intros prefix ns tr H.
+  rewrite foo in H. rewrite app_nil_l in H. subst.
+  rewrite foo. reflexivity.
+Qed.
+
+
+
+
+Inductive Instr : Set :=
+| hash : Instr.
+
+Inductive AnnoInstr : Type :=
+| aprimInstr: nat -> Instr -> AnnoInstr.
+
+Fixpoint instr_compiler (t:AnnoTerm) : (list AnnoInstr) :=
+  match t with
+  | aasp r a => [aprimInstr (fst r) (asp_instr a)]  
+(*  | aatt r q t' => [areqrpy r q t']      *)        
+  | alseq _ t1 t2 =>
+    let tr1 := instr_compiler t1 in
+    let tr2 := instr_compiler t2 in
+    tr1 ++ tr2 
+
